split checkLevel and checkRoot
Signed-off-by: John Kastner <jkastner@amazon.com>

cedar-lean/Cedar/Validation/Levels.lean
@@ -42,78 +42,70 @@ structure LevelCheckResult where
 
 def LevelCheckResult.and (r₀ r₁ : LevelCheckResult) : LevelCheckResult := LevelCheckResult.mk (r₀.checked && r₁.checked) (r₀.root && r₁.root)
 
-def checkLevel (tx : TypedExpr) (n : Nat) : LevelCheckResult :=
+def checkRoot : TypedExpr → Bool
+  | .lit _ _ => false
+  | .ite _ x₂ x₃ _ =>
+    checkRoot x₂ && checkRoot x₃
+  | .getAttr x₁ _ _
+  | .binaryApp .getTag x₁ _ _ =>
+    checkRoot x₁
+  | .set xs _ =>
+    xs.attach.all λ x =>
+      have := List.sizeOf_lt_of_mem x.property
+      checkRoot x
+  | .record axs _ =>
+    axs.attach.all λ e =>
+      have : sizeOf e.val.snd < 1 + sizeOf axs := by
+        have h₁ := List.sizeOf_lt_of_mem e.property
+        rw [Prod.mk.sizeOf_spec e.val.fst e.val.snd] at h₁
+        omega
+      checkRoot e.val.snd
+  | _ => true
+
+def checkLevel (tx : TypedExpr) (n : Nat) : Bool :=
   match tx with
-  | .lit _ _ => LevelCheckResult.mk true false
-  | .var _ _ => LevelCheckResult.mk true true
+  | .lit _ _ => true
+  | .var _ _ => true
   | .ite x₁ x₂ x₃ _ =>
-    let c₁ := checkLevel x₁ n
-    let c₂ := checkLevel x₂ n
-    let c₃ := checkLevel x₃ n
-    LevelCheckResult.mk
-      (c₁.checked && c₂.checked && c₃.checked)
-      (c₂.root && c₃.root)
+    checkLevel x₁ n &&
+    checkLevel x₂ n &&
+    checkLevel x₃ n
   | .unaryApp _ x₁ _ =>
     checkLevel x₁ n
   | .binaryApp .mem x₁ x₂ _
   | .binaryApp .getTag x₁ x₂ _
   | .binaryApp .hasTag x₁ x₂ _ =>
-    let c₁ := checkLevel x₁ (n - 1)
-    let c₂ := checkLevel x₂ n
-    LevelCheckResult.mk
-      (c₁.root && n > 0 && c₁.checked && c₂.checked)
-      c₁.root
+    checkRoot x₁ &&
+    n > 0 &&
+    checkLevel x₁ (n - 1) &&
+    checkLevel x₂ n
   | .and x₁ x₂ _
   | .or x₁ x₂ _
   | .binaryApp _ x₁ x₂ _ =>
-    let c₁ := checkLevel x₁ n
-    let c₂ := checkLevel x₂ n
-    LevelCheckResult.mk
-      (c₁.checked && c₂.checked)
-      true
+    checkLevel x₁ n &&
+    checkLevel x₂ n
   | .hasAttr x₁ _ _
   | .getAttr x₁ _ _ =>
     match x₁.typeOf with
     | .entity _ =>
-      let c₁ := checkLevel x₁ (n - 1)
-      LevelCheckResult.mk
-        (c₁.root && n > 0 && c₁.checked)
-        c₁.root
-    | _ => (checkLevel x₁ n)
+      checkRoot x₁ &&
+      n > 0 &&
+      checkLevel x₁ (n - 1)
+    | _ => checkLevel x₁ n
   | .call _ xs _
   | .set xs _ =>
-    xs.attach.foldl
-      (λ c ex =>
-        have := List.sizeOf_lt_of_mem ex.property
-        let c₁ := checkLevel ex.val n
-        LevelCheckResult.mk
-          (c.checked && c₁.checked)
-          (c.root && c₁.root))
-      (LevelCheckResult.mk true true)
+    xs.attach.all λ e =>
+      have := List.sizeOf_lt_of_mem e.property
+      checkLevel e n
   | .record axs _ =>
-    axs.attach.foldl
-      (λ c a =>
-        let t := a.val.snd
-        --have : sizeOf t < 1 + sizeOf axs := by
-        --  have : t = a.val.snd := by simp [t]
-        --  rw [this]
-        --  have h₁ := List.sizeOf_lt_of_mem a.property
-        --  rw [Prod.mk.sizeOf_spec a.val.fst a.val.snd] at h₁
-        --  omega
-        let c₁ := checkLevel a.val.snd n
-        LevelCheckResult.mk
-          (c.checked && c₁.checked)
-          (c.root && c₁.root))
-      (LevelCheckResult.mk true true)
-  termination_by tx
-  decreasing_by
-    all_goals {
-      try { simp ; omega }
-      -- TODO: Record case doesn't go through after changing from `all` to `foldl`
-      try sorry
-    }
+    axs.attach.all λ e =>
+      have : sizeOf e.val.snd < 1 + sizeOf axs := by
+        have h₁ := List.sizeOf_lt_of_mem e.property
+        rw [Prod.mk.sizeOf_spec e.val.fst e.val.snd] at h₁
+        omega
+      checkLevel e.val.snd n
 
 def typedAtLevel (e : Expr) (c : Capabilities) (env : Environment) (n : Nat) : Bool :=
   match typeOf e c env with
-  | .ok (te, _) => (checkLevel te n).checked
+  | .ok (te, _) => checkLevel te n
   | _           => false
