cedar-lean/Cedar/Thm/Validation/Levels/Basic.lean
@@ -30,5 +30,5 @@ def TypedAtLevelIsSound (e : Expr) : Prop := ∀ {n : Nat} {tx : TypedExpr} {c c
   CapabilitiesInvariant c request entities →
   RequestAndEntitiesMatchEnvironment env request entities →
   typeOf e c env = Except.ok (tx, c₁) →
-  (checkLevel tx n).checked →
+  checkLevel tx n →
   evaluate e request entities = evaluate e request slice
